\documentclass{article}

\usepackage{todonotes}

\addtolength{\oddsidemargin}{-.875in}
\addtolength{\evensidemargin}{-.875in}
\addtolength{\textwidth}{1.75in}

\addtolength{\topmargin}{-.875in}
\addtolength{\textheight}{1.75in}

\bibliographystyle{plain}

\begin{document}
\title{An Introduction to The Lambda Calculus}
\author{Erik Boesen}
\maketitle
\todo{Consider more specific title}
\begin{abstract}
\end{abstract}

\section{What is the Lambda Calculus?}
The lambda calculus (hereinafter notated as ``the $\lambda$-calculus'') is a system of mathematical notation and logic developed for the study of the elementary properties of functions \cite{rojastutorial}.

The notation and concept of the $\lambda$-calculus was first described in 1930 by Alonzo Church \cite{church}.\footnote{It underwent revisions following criticism as logically invalid \cite{church2}.} The system can be used to represent any computation traditionally possible. So, it is equivalent in capability to a ``Turing machine''â€”a mathematical notion of a computer.

Later, the system of notation gained new notoriety as the basis for new forms of computer programming. The $\lambda$-calculus is sometimes referred to as a universal programming language \cite{rojastutorial}, given that it can represent and perform the computations of a Turing machine and vice versa. The $\lambda$-calculus is the basis for functional programming languages, or those whose attributes including treating functions as data and using a declarative programming paradigm \cite{hudakevolution}. The topic of functional programming is beyond the scope of this paper, however, interested readers are invited to investigate the topic through papers including \cite{totalfp} and \cite{hudakevolution}.

\section{Notation}
The notation used to describe $\lambda$-calculus expressions seldom bears resemblance to more traditional systems of mathematical notation. To describe, for instance, the identity function (in which a single parameter is given as input and is outputted without modification) in traditional notation, one would likely use some variation upon:
$$f(x)=x$$
To make the function anonymous in traditional notation, one could use:
$$(x) \mapsto x$$
In the $\lambda$-calculus, however, an anonymous identity function would be notated thus:
$$\lambda x.x$$
Lambda calculus expressions associate left-to-right. So, Lambda expressions can be applied simply by parenthesizing them and appending parameters afterward. So, to apply our identity function to some constant $C$, we would perform the following lambda computation:
$$(\lambda x.x)C$$
$$=\lambda x.C$$
$$=C$$
Some explanation of the symbolic logic used herein is in order. Only two symbols in the calculus are defined, $\lambda$ and $.$ (some other symbols, such as parentheses, are used intuitively for grouping and other purposes). The former is used to represent a function definition, whereas the latter separates parameters from that function's internal logic. The sum of those two components is referred to as an ``abstraction.'' The $\lambda$-calculus also defines ``applications,'' or one lambda expression applied to another \cite{horowitz}.

The important thing to note about the aforementioned syntax is that in pure $\lambda$-calculus, there are no other symbols or gramatical constructions used. This leads to some occasionally verbose definitions for otherwise simple concepts. Basic mathematical functions are generally defined through several facilities. The first important thing to know in order to redefine things like addition is the ``successor'' function:
$$$$


Throughout this paper, we will generally try to keep to the pure $\lambda$-calculus where possible, however, given that this is typically inconvenient,

\section{Currying}
The $\lambda$-calculus' syntax for representation of multi-parameter functions is potentially surprising. Purely speaking, there is no notion of multi-parameter functions. Rather, the $\lambda$-calculus makes use of ``currying,'' a technique named after mathematician Haskell Curry. In this process, a function which would typically require multiple parameters transforms into a series of functions requiring only one parameter each. So,
$$\lambda xyz.x+y+z$$\todo{Use pure equation somehow?}
would expand to
$$\lambda x.\lambda y.\lambda z.x+y+z$$
These two expressions are equivalent, assuming that the impure syntax used in the first represents one function with three parameters $x$, $y$, and $z$. Let us see how this expression would be applied:
$$(\lambda x.\lambda y.\lambda z.x+y+z)ABC$$
The outer function would be applied first, and the single parameter it accepts, $x$, would be substituted into the body\todo{Right name?} of the enclosed function. So, the above expression would first simplify to:
$$(\lambda y.\lambda z.A+y+z)BC$$
$$(\lambda z.A+B+z)C$$
$$A+B+C$$

\section{Recursion and the Y Combinator}

\bibliography{research}
\end{document}
